Work on updating MontgomeryLadder NOTE: does not build

src/Bedrock/Group/ScalarMult/MontgomeryLadder.v
@@ -14,6 +14,27 @@ Require Import Crypto.Bedrock.Specs.ScalarField.
 Require Import Crypto.Util.NumTheoryUtil.
 Local Open Scope Z_scope.
 
+
+Notation "'let/n' ( w , x , y , z ) := val 'in' body" :=
+  (nlet [IdentParsing.TC.ident_to_string w;
+        IdentParsing.TC.ident_to_string x;
+        IdentParsing.TC.ident_to_string y;
+        IdentParsing.TC.ident_to_string z]
+        val  (fun '(w, x, y, z) => body))
+   (at level 200, w ident, x  ident, y ident, z ident, body at level 200,
+    only parsing).
+
+Notation "'let/n' ( v , w , x , y , z ) := val 'in' body" :=
+  (nlet [IdentParsing.TC.ident_to_string v;
+        IdentParsing.TC.ident_to_string w;
+        IdentParsing.TC.ident_to_string x;
+        IdentParsing.TC.ident_to_string y;
+        IdentParsing.TC.ident_to_string z]
+        val  (fun '(v, w, x, y, z) => body))
+   (at level 200, v ident,  w ident, x  ident, y ident, z ident, body at level 200,
+     only parsing).
+
+
 Section __.
   Context {width: Z} {BW: Bitwidth width} {word: word.word width} {mem: map.map word Byte.byte}.
   Context {locals: map.map String.string word}.
@@ -37,27 +58,34 @@ Section __.
     Definition montladder_gallina
                (scalarbits : Z) (testbit:nat ->bool) (u:F M_pos)
       : F M_pos :=
-      let/n P1 := (1, 0) in
-      let/n P2 := (u, 1) in
+      let/n X1 := felem_alloc 1 in
+      let/n Z1 := felem_alloc 0 in
+      let/n X2 := felem_alloc u in
+      let/n Z2 := felem_alloc 1 in
+     (* let/d P1 := (1, 0) in
+        let/d P2 := (X2, Z2) in
+      *)
       let/n swap := false in
       let/n count := scalarbits in
-      let '(P1, P2, swap) :=
+      let/n (X1, Z1, X2, Z2, swap) :=
          downto
-           (P1, P2, swap) (* initial state *)
+           (X1, Z1, X2, Z2, swap) (* initial state *)
            (Z.to_nat count)
            (fun state i =>
-              let '(P1, P2, swap) := state in
+              (*TODO: should this be a /n?*)
+              let '(X1, Z1, X2, Z2, swap) := state in
               let/n s_i := testbit i in
               let/n swap := xorb swap s_i in
-              let/n (P1, P2) := cswap swap P1 P2 in
-              let/n (P1, P2) := ladderstep_gallina u P1 P2 in
+              let/n (X1, X2) := cswap swap X1 X2 in
+              let/n (Z1, Z2) := cswap swap Z1 Z2 in
+              let/n (X1, Z1, X2, Z2) := ladderstep_gallina u X1 Z1 X2 Z2 in
               let/n swap := s_i in
-              (P1, P2, swap)
+              (X1, Z1, X2, Z2, swap)
            ) in
-      let/n (P1, P2) := cswap swap P1 P2 in
-      let '(x, z) := P1 in
-      let/n r := F.inv z in
-      let/n r := (x * r) in
+      let/n (X1, X2) := cswap swap X1 X2 in
+      let/n (Z1, Z2) := cswap swap Z1 Z2 in
+      let/n r := F.inv Z1 in
+      let/n r := (X1 * r) in
       r.
   End Gallina.
 
@@ -66,25 +94,19 @@ Section __.
 
     Instance spec_of_montladder : spec_of "montladder" :=
       fnspec! "montladder"
-            (pOUT pK pU pX1 pZ1 pX2 pZ2
-                  pA pAA pB pBB pE pC pD pDA pCB : word)
+            (pOUT pK pU (*pX1 pZ1 pX2 pZ2*) : Semantics.word)
             / (K : scalar) (U : felem) (* inputs *)
-            OUT X1 Z1 X2 Z2 A AA B BB E C D DA CB (* intermediates *)
+            OUT (*X1 Z1 X2 Z2 *) (* intermediates *)
             R,
       { requires tr mem :=
            bounded_by tight_bounds U
            /\ (FElem pOUT OUT * Scalar pK K * FElem pU U
-               * FElem pX1 X1 * FElem pZ1 Z1
-               * FElem pX2 X2 * FElem pZ2 Z2
-               * FElem pA A * FElem pAA AA
-               * FElem pB B * FElem pBB BB
-               * FElem pE E * FElem pC C
-               * FElem pD D * FElem pDA DA
-               * FElem pCB CB * R)%sep mem;
+              (** FElem pX1 X1 * FElem pZ1 Z1
+               * FElem pX2 X2 * FElem pZ2 Z2*)
+               *  R)%sep mem;
         ensures tr' mem' :=
           tr' = tr
-          /\ (exists OUT X1 Z1 X2 Z2
-                     A AA B BB E C D DA CB : felem,
+          /\ (exists OUT (*X1 Z1 X2 Z2*)  : felem,
                  feval OUT = montladder_gallina
                                scalarbits
                                (fun i =>
@@ -93,13 +115,10 @@ Section __.
                                (feval U)
             /\ bounded_by tight_bounds OUT
             /\ (FElem pOUT OUT * Scalar pK K * FElem pU U
-                * FElem pX1 X1 * FElem pZ1 Z1
-                * FElem pX2 X2 * FElem pZ2 Z2
-                * FElem pA A * FElem pAA AA
-                * FElem pB B * FElem pBB BB
-                * FElem pE E * FElem pC C
-                * FElem pD D * FElem pDA DA
-                * FElem pCB CB * R)%sep mem) }.
+                (** FElem pX1 X1 * FElem pZ1 Z1
+                * FElem pX2 X2 * FElem pZ2 Z2 *)
+                * R)%sep mem') }.
+
 
     Ltac apply_compile_cswap_nocopy :=
       simple eapply compile_cswap_nocopy with
@@ -132,26 +151,20 @@ Section __.
             | apply_compile_cswap_nocopy ].
 
     (* TODO: make a new loop invariant, drop the sep-local stuff *)
-    (*
+    (*nat -> bool -> F M_pos * F M_pos * F M_pos * F M_pos * bool -> predicate*)
     Definition downto_inv
-               swap_var X1_var Z1_var X2_var Z2_var K_var
-               K K_ptr X1_ptr Z1_ptr X2_ptr Z2_ptr Rl
-               A_ptr AA_ptr B_ptr BB_ptr E_ptr C_ptr D_ptr DA_ptr CB_ptr
-               (locals : Semantics.locals)
+               (swap_var  X1_var Z1_var X2_var Z2_var K_var : string)
+               K (K_ptr X1_ptr Z1_ptr X2_ptr Z2_ptr : word) R
                (_ : nat)
                (gst : bool)
-               (st : point * point * bool)
-               (_ : list word)
-      : Semantics.mem -> Prop :=
-      let P1 := fst (fst st) in
-      let P2 := snd (fst st) in
-      let swap := snd st in
-      let x1 := fst P1 in
-      let z1 := snd P1 in
-      let x2 := fst P2 in
-      let z2 := snd P2 in
+               (st : F M_pos * F M_pos * F M_pos * F M_pos * bool)
+      : predicate :=
+      fun (_ : Semantics.trace)
+          (mem : Semantics.mem)
+          (locals : Semantics.locals) =>
+      let '(x1, z1, x2, z2, swap) := st in
       let swapped := gst in
-      liftexists X1_ptr' Z1_ptr' X2_ptr' Z2_ptr'
+      (liftexists X1_ptr' Z1_ptr' X2_ptr' Z2_ptr'
                  X1 Z1 X2 Z2,
         (emp (bounded_by tight_bounds X1
               /\ bounded_by tight_bounds Z1
@@ -161,7 +174,7 @@ Section __.
               /\ feval Z1 = z1
               /\ feval X2 = x2
               /\ feval Z2 = z2
-              /\ (if swapped
+            (* /\ (if swapped
                   then (X1_ptr' = X2_ptr
                         /\ Z1_ptr' = Z2_ptr
                         /\ X2_ptr' = X1_ptr
@@ -173,19 +186,14 @@ Section __.
               /\ (Var swap_var (word.of_Z (Z.b2z swap)) * Var K_var K_ptr
                   * Var X1_var X1_ptr' * Var Z1_var Z1_ptr'
                   * Var X2_var X2_ptr' * Var Z2_var Z2_ptr'
-                  * Rl)%sep locals)
+                  * Rl)%sep locals *) )
          * (Scalar K_ptr K * FElem X1_ptr' X1 * FElem Z1_ptr' Z1
-            * FElem X2_ptr' X2 * FElem Z2_ptr' Z2
-            * Placeholder A_ptr * Placeholder AA_ptr
-            * Placeholder B_ptr * Placeholder BB_ptr
-            * Placeholder E_ptr * Placeholder C_ptr
-            * Placeholder D_ptr * Placeholder DA_ptr
-            * Placeholder CB_ptr))%sep.
-*)
+            * FElem X2_ptr' X2 * FElem Z2_ptr' Z2) * R)%sep) mem.
+
     Definition downto_ghost_step
-               (K : scalar) (st : point * point * bool)
+               (K : scalar) (st : F M_pos * F M_pos * F M_pos * F M_pos * bool)
                (gst : bool) (i : nat) :=
-      let swap := snd st in
+      let '(x1, z1, x2, z2, swap) := st in
       let swap := xorb swap (Z.testbit (F.to_Z (sceval K)) (Z.of_nat i)) in
       xorb gst swap.
 
@@ -285,10 +293,296 @@ Section __.
 
     Existing Instance spec_of_sctestbit.
 
-    Local Hint Extern 1 (spec_of _) => (simple refine (@spec_of_felem_small_literal _ _ _ _ _ _ _ _)) : typeclass_instances.
+
+      Lemma compile_felem_small_literal_alloc {tr mem locals functions} x:
+    let v := felem_alloc (F.of_Z _ x) in
+    forall {P} {pred: P v -> predicate} {k: nlet_eq_k P v} {k_impl}
+      (R : _ -> Prop) (wx : word) out_var,
+
+      spec_of_felem_small_literal functions ->
+      R mem ->
+
+      word.unsigned wx = x ->
+
+      (let v := v in
+       forall X m out_ptr,
+         (FElem out_ptr X * R)%sep m ->
+         feval X = v ->
+         bounded_by tight_bounds X ->
+         (<{ Trace := tr;
+             Memory := m;
+             Locals := map.put locals out_var out_ptr;
+             Functions := functions }>
+          k_impl
+          <{ pred_sep (Placeholder out_ptr) pred (k v eq_refl) }>)) ->
+      <{ Trace := tr;
+         Memory := mem;
+         Locals := locals;
+         Functions := functions }>
+      cmd.stackalloc out_var (@felem_size_in_bytes field_parameters _ field_representaton)
+                     (cmd.seq
+                        (cmd.call [] felem_small_literal
+                                  [expr.var out_var; expr.literal x])
+                        k_impl)
+      <{ pred (nlet_eq [out_var] v k) }>.
+  Proof.
+     repeat straightline'.
+     split; eauto using felem_size_in_bytes_mod.
+     intros out_ptr mStack mCombined Hplace%FElem_from_bytes.
+     destruct Hplace as [out Hout].
+     repeat straightline'.
+     straightline_call.
+     intuition eauto.
+     {
+       exists mStack.
+       exists mem.
+       intuition eauto.
+       apply map.split_comm; eauto.
+     }
+     repeat straightline'.
+     eapply WeakestPrecondition_weaken
+       with (p1 := pred_sep (Memory.anybytes out_ptr felem_size_in_bytes)
+                            pred (let/n x as out_var eq:Heq := v in
+                                  k x Heq)).
+     {
+       unfold pred_sep.
+       repeat straightline'.
+       destruct H4 as [mStack' [m' [Hmem [HmStack Hm]]]].
+       unfold Basics.flip in Hm.
+       exists m'.
+       exists mStack'.
+       intuition.
+       apply map.split_comm; auto.
+     }
+     eapply H2; repeat straightline'.
+     {
+       unfold v.
+       unfold felem_alloc.
+       eauto.
+     }
+     eauto.
+     {
+       rewrite H6.
+       rewrite <- H1.
+       rewrite word.of_Z_unsigned.
+       rewrite H1.
+       reflexivity.
+     }
+     eauto.
+  Qed.
+
+  
+  Lemma compile_felem_copy_alloc {tr mem locals functions} x :
+    let v := feval x in
+    forall {P} {pred: P v -> predicate} {k: nlet_eq_k P v} {k_impl}
+      R x_ptr x_var out_var,
+
+      spec_of_felem_copy functions ->
+
+      (FElem x_ptr x  * R)%sep mem ->
+      map.get locals x_var = Some x_ptr ->
+
+      out_var<> x_var ->
+      
+      (let v := v in
+       forall X m out_ptr,
+         (FElem out_ptr X * (FElem x_ptr x  * R))%sep m ->
+         feval X = v ->
+         (<{ Trace := tr;
+             Memory := m;
+             Locals := map.put locals out_var out_ptr;
+             Functions := functions }>
+          k_impl
+          <{ pred_sep (Placeholder out_ptr) pred (k v eq_refl) }>)) ->
+      <{ Trace := tr;
+         Memory := mem;
+         Locals := locals;
+         Functions := functions }>
+      cmd.stackalloc out_var (@felem_size_in_bytes field_parameters _ field_representaton)
+      (cmd.seq
+        (cmd.call [] felem_copy [expr.var out_var; expr.var x_var])
+        k_impl)
+      <{ pred (nlet_eq [out_var] v k) }>.
+  Proof.
+     repeat straightline'.
+     split; eauto using felem_size_in_bytes_mod.
+     intros out_ptr mStack mCombined Hplace%FElem_from_bytes.
+     destruct Hplace as [out Hout].
+     repeat straightline'.
+     straightline_call.
+     intuition eauto.
+     {
+       apply sep_assoc.
+       apply sep_comm.
+       apply sep_assoc.
+       exists mStack.
+       exists mem.
+       intuition eauto.
+       eauto.
+       apply map.split_comm; eauto.
+       apply sep_comm; eauto.
+     }
+     repeat straightline'.
+     eapply WeakestPrecondition_weaken
+       with (p1 := pred_sep (Memory.anybytes out_ptr felem_size_in_bytes)
+                            pred (let/n x as out_var eq:Heq := v in
+                                  k x Heq)).
+     {
+       unfold pred_sep.
+       repeat straightline'.
+       destruct H5 as [mStack' [m' [Hmem [HmStack Hm]]]].
+       unfold Basics.flip in Hm.
+       exists m'.
+       exists mStack'.
+       intuition.
+       apply map.split_comm; auto.
+     }
+     eapply H3; repeat straightline'.
+     {
+       unfold v.
+       unfold felem_alloc.
+       ecancel_assumption.
+     }
+     eauto.
+  Qed.
+
+  (*TODO: why doesn't simple eapply work? *)
+Ltac field_compile_step ::=
+  first [ simple eapply compile_scmula24 (* must precede compile_mul *)
+        | simple eapply compile_mul
+        | simple eapply compile_add
+        | simple eapply compile_sub
+        | simple eapply compile_square
+        | simple eapply compile_inv
+        (*must come second due to eapply *)
+        | eapply compile_scmula24_alloc (* must precede compile_mul_alloc *)
+        | eapply compile_mul_alloc
+        | eapply compile_add_alloc
+        | eapply compile_sub_alloc
+        | eapply compile_square_alloc
+        | eapply compile_inv_alloc 
+        | eapply compile_felem_small_literal_alloc
+        | eapply compile_felem_copy_alloc ];
+  lazymatch goal with
+  | |- feval _ = _ => try eassumption; try reflexivity
+  | |- _ => idtac
+  end.
+
+
+  
+  Ltac ladderstep_compile_custom :=
+    simple apply compile_nlet_as_nlet_eq;
+    field_compile_step; [ repeat compile_step .. | intros ];
+    eauto with compiler;
+    (* rewrite results in terms of feval to match lemmas *)
+    repeat lazymatch goal with
+           | H : feval _ = ?x |- context [?x] =>
+             is_var x; rewrite <-H
+           end.
+  
+  Ltac compile_custom ::= ladderstep_compile_custom.
+
+
+  
+  (*TODO: move to right place*)
+  (* There are two ways cswap could be compiled; you can either swap the local
+     variables (the pointers), or you can leave the pointers and copy over the
+     data. This version does the copying. *)
+  Lemma compile_cswap_nocopy {tr mem locals functions} (swap: bool) {A} (x y: A) :
+    let v := cswap swap x y in
+    forall {P} {pred: P v -> predicate}
+      {k: nlet_eq_k P v} {k_impl}
+      R (Data : word -> A -> Semantics.mem -> Prop)
+      swap_var x_var x_ptr y_var y_ptr tmp,
+
+      map.get locals swap_var = Some (word.of_Z (Z.b2z swap)) ->
+      map.get locals x_var = Some x_ptr ->
+      map.get locals y_var = Some y_ptr ->
+
+      (* tmp is a strictly temporary variable, confined to one part of the
+         if-clause; it gets unset after use *)
+      map.get locals tmp = None ->
+      (Data x_ptr x * Data y_ptr y * R)%sep mem ->
+
+      (let v := v in
+       <{ Trace := tr;
+          Memory := mem;
+          Locals := map.put (map.put locals x_var (fst (cswap swap x_ptr y_ptr))) y_var
+                      (snd (cswap swap x_ptr y_ptr));
+          Functions := functions }>
+       k_impl
+       <{ pred (k v eq_refl) }>) ->
+      <{ Trace := tr;
+         Memory := mem;
+         Locals := locals;
+         Functions := functions }>
+      cmd.seq
+        (cmd.cond
+           (expr.var swap_var)
+           (cmd.seq
+              (cmd.seq
+                 (cmd.seq
+                    (cmd.set tmp (expr.var x_var))
+                    (cmd.set x_var (expr.var y_var)))
+                 (cmd.set y_var (expr.var tmp)))
+              (cmd.unset tmp))
+           (cmd.skip))
+        k_impl
+      <{ pred (nlet_eq [x_var; y_var] v k) }>.
+  Proof.
+    intros; subst v; unfold cswap.
+    simple eapply compile_if with
+        (val_pred := fun _ tr' mem' locals' =>
+                      tr' = tr /\
+                      mem' = mem /\
+                      locals' =
+                      let locals := map.put locals x_var (if swap then y_ptr else x_ptr) in
+                      let locals := map.put locals y_var (if swap then x_ptr else y_ptr) in
+                      locals);
+      repeat compile_step;
+      repeat straightline'; subst_lets_in_goal; cbn; ssplit; eauto.
+    - rewrite !map.remove_put_diff, !map.remove_put_same, map.remove_not_in by congruence.
+      reflexivity.
+    - rewrite (map.put_noop x_var x_ptr), map.put_noop by assumption.
+      reflexivity.
+    - cbv beta in *; repeat compile_step; cbn.
+      destruct swap; eassumption.
+  Qed.
+
+  
+  Lemma compile_cswap_pair {tr mem locals functions} (swap: bool) {A} (x y: A * A) x1 x2 :
+    let v := cswap swap x y in
+    forall {P} {pred: P v -> predicate}
+      {k: nlet_eq_k P v} {k_impl},
+      (let __ := 0 in (* placeholder FIXME why? *)
+       <{ Trace := tr;
+          Memory := mem;
+          Locals := locals;
+          Functions := functions }>
+       k_impl
+       <{ pred (nlet_eq [x1] (cswap swap (fst x) (fst y))
+                     (fun xy1 eq1 =>
+                        nlet_eq [x2] (cswap swap (snd x) (snd y))
+                             (fun xy2 eq2 =>
+                                let x := (fst xy1, fst xy2) in
+                                let y := (snd xy1, snd xy2) in
+                                k (x, y) ltac:(eauto)))) }>) ->
+      <{ Trace := tr;
+         Memory := mem;
+         Locals := locals;
+         Functions := functions }>
+      k_impl
+      <{ pred (nlet_eq [x1; x2] v k) }>.
+  Proof.
+    repeat straightline'.
+    subst_lets_in_goal. destruct_products.
+    destruct swap; cbv [cswap dlet] in *; cbn [fst snd] in *.
+    all:eauto.
+  Qed.
+
+
     Derive montladder_body SuchThat
-           (let args := ["OUT"; "K"; "U"; "X1"; "Z1"; "X2"; "Z2";
-                           "A"; "AA"; "B"; "BB"; "E"; "C"; "D"; "DA"; "CB"] in
+           (let args := ["OUT"; "K"; "U" (*;"X1"; "Z1"; "X2"; "Z2" *)] in
             let montladder : Syntax.func :=
                 ("montladder", (args, [], montladder_body)) in
           ltac:(
@@ -298,6 +592,223 @@ Section __.
             exact (__rupicola_program_marker montladder_gallina -> goal)))
          As montladder_correct.
     Proof.
+      pose proof scalarbits_pos.
+      pose proof unsigned_of_Z_1.
+      pose proof unsigned_of_Z_0.
+      compile_setup.
+      unfold F.one.
+      unfold F.zero.
+      compile_step.
+      compile_step.
+      compile_step.
+      compile_step.
+      compile_step.
+      compile_step.
+      compile_step.
+      compile_step.
+      compile_step.
+      compile_step.
+      simple apply compile_nlet_as_nlet_eq.
+      let tmp_var := constr:("tmp") in
+      let x1_var := constr:("X1") in
+      let z1_var := constr:("Z1") in
+      let x2_var := constr:("X2") in
+      let z2_var := constr:("Z2") in
+      let counter_var := constr:("count") in
+      eapply compile_downto with (i_var := counter_var)
+      (wcount := word.of_Z scalarbits)
+      (ginit := false)
+      (ghost_step := downto_ghost_step K)
+      (Inv :=
+         downto_inv
+           _ x1_var z1_var x2_var z2_var _
+           _ pK out_ptr out_ptr0 out_ptr1 out_ptr2
+           _).
+      {
+        unfold downto_inv.
+        repeat compile_step.
+        exists out_ptr.
+        exists out_ptr0.
+        exists out_ptr1.
+        exists out_ptr2.
+        exists X.
+        exists X0.
+        exists X1.
+        exists X2.
+        progress sepsimpl; eauto.
+        admit(*TODO: why no bounds for X1?*).
+        (*instantiate (3:="count").*)
+        (*instantiate (2:="K").*)
+(*        admit.*)
+        ecancel_assumption.
+      }
+      compile_step.
+      admit (*z/word math*).
+      lia.
+      {
+        compile_step.
+        unfold downto_inv in H11.
+        repeat destruct st as [st ?].
+        do 8 destruct H11 as [? H11].
+        sepsimpl.
+        eapply compile_nlet_as_nlet_eq.
+        eapply compile_sctestbit; eauto.
+        ecancel_assumption.
+        instantiate (1:="K"); admit (*TODO: need pK in locals; add to downto_inv?*).
+        compile_step.
+        repeat compile_step.
+        admit(*TODO: what is b? also from inv?*).
+        repeat compile_step.
+        
+
+
+
+Locate "let/n".
+
+
+
+
+
+        
+        (*TODO: update cswap lemma*)
+        eapply  compile_cswap_pair; eauto.
+        admit (*map_get*).
+        exact H11.
+        intros. clear_old_seps.
+        match goal with gst' := downto_ghost_step _ _ _ _ |- _ =>
+                                subst gst' end.
+        destruct_products.
+        cbv [downto_inv] in * |-. sepsimpl_hyps.
+        eexists; intros.
+
+        (* convert locals back to literal map using the separation-logic
+           condition; an alternative would be to have all lemmas play nice with
+           locals in separation logic *)
+        match goal with H : sep _ _ (map.remove _ ?i_var)
+                        |- context [map.get _ ?i_var = Some ?wi] =>
+                        eapply Var_put_remove with (v:=wi) in H;
+                          eapply sep_assoc in H
+        end.
+        literal_locals_from_sep.
+        unfold downto_inv in *.
+        repeat destruct st as [st ?].
+        simpl in *.
+        do 8 destruct H11 as [? H11].
+        sepsimpl.
+        eapply compile_nlet_as_nlet_eq.
+        simpl.
+        compile_step.
+        TODO: no R
+        simpl.
+        
+      let locals := lazymatch goal with
+                    | |- WeakestPrecondition.cmd _ _ _ _ ?l _ => l end in
+        simple eapply compile_downto with
+            (wcount := word.of_Z scalarbits)
+            (ginit := false)
+            (i_var := counter_var)
+            (ghost_step := downto_ghost_step K)
+          (*  (Inv :=
+               downto_inv
+                 _ x1_var z1_var x2_var z2_var _
+                 _ pK pX1 pZ1 pX2 pZ2
+                 _ pA pAA pB pBB pE pC pD pDA pCB);
+          [ .. | subst L | subst L ].*).
+      eapply compile_downto.
+      eapply
+      simple apply compile_nlet_as_nlet_eq.
+      compile_step.
+      repeat compile_step.
+      {
+        unfold pred_sep; simpl.
+        unfold Basics.flip; simpl.
+        repeat change (fun x => ?h x) with h.
+        unfold map.getmany_of_list.
+        simpl.
+        {
+          (*TODO: do in a better way*)
+          change (fun y => exists ws, @?P ws y) with (Lift1Prop.ex1 P).
+          repeat seprewrite FElem_from_bytes.
+          repeat (sepsimpl;
+                  match goal with
+                    [H : context [FElem ?p ?v] |- Lift1Prop.ex1 (fun h => FElem ?p h * _)%sep _] =>
+                    exists v
+                  end).
+          sepsimpl.
+          exists [].
+          cbv beta.
+          eapply Proper_sep_iff1.
+          2: reflexivity.
+          {
+            instantiate (1:=
+                           Lift1Prop.ex1 (fun OUT0 =>
+                                            feval OUT0 =
+        (let
+         '(X4, Z1, X3, Z2, swap) :=
+          downto (feval X, feval X0, feval X1, feval X2, false) (Z.to_nat scalarbits)
+            (fun (state : F M_pos * F M_pos * F M_pos * F M_pos * bool) (i : nat) =>
+             let
+             '(X4, Z1, X3, Z2, swap) := state in
+              let/n s_i as "s_i" := Z.testbit (F.to_Z (sceval K)) (Z.of_nat i) in
+              let/n swap0 as "swap" := xorb swap s_i in
+              let/n (X5, X6) as ("X1", "X2") := cswap swap0 X4 X3 in
+              let/n (Z0, Z3) as ("Z1", "Z2") := cswap swap0 Z1 Z2 in
+              nlet ["X1"; "Z1"; "X2"; "Z2"] (ladderstep_gallina (feval U) X5 Z0 X6 Z3)
+                (fun '(X8, Z5, X7, Z4) => let/n x as "swap" := s_i in
+                                          (X8, Z5, X7, Z4, x))) in
+          let/n (X5, _) as ("X1", "X2") := cswap swap X4 X3 in
+          let/n (Z0, _) as ("Z1", "Z2") := cswap swap Z1 Z2 in
+          let/n r as "r" := F.inv Z0 in
+          let/n r0 as "r" := (X5 * r)%F in
+          r0) /\ bounded_by tight_bounds OUT0 /\ (FElem pOUT OUT0 ⋆ Scalar pK K ⋆ FElem pU U ⋆ R) y)).
+            simpl.
+            instantiate (1:=
+                       (Lift1Prop.ex1 (fun X4 =>
+                        Lift1Prop.ex1 (fun Z4 =>
+                        Lift1Prop.ex1 (fun X5 =>
+                        Lift1Prop.ex1 (fun Z5 =>
+                        (emp ((feval out13, feval out16, feval out9, feval out12)
+                         = (feval X4, feval Z4, feval X5, feval Z5) /\
+                        bounded_by tight_bounds X4 /\
+                        bounded_by tight_bounds Z4 /\
+                        bounded_by tight_bounds X5 /\ bounded_by tight_bounds Z5))
+                        * (FElem pX1 X1 ⋆ FElem pX2 X4 ⋆ FElem pZ2 Z4 ⋆ FElem pX3 X5 ⋆ FElem pZ3 Z5 ⋆ R))))))%sep).
+        cbv [Lift1Prop.iff1 Lift1Prop.ex1].
+        intuition idtac.
+        {
+          destruct H33 as (?&?&?&?&?).
+          exists x0, x1, x2, x3.
+          intuition idtac.
+          eapply sep_emp_l.
+          intuition idtac.
+        }
+        {
+          destruct H28 as (?&?&?&?&?).
+          exists x0, x1, x2, x3.
+          eapply sep_emp_l in H28.
+          intuition idtac.
+        }
+      }
+      sepsimpl; eexists.
+      sepsimpl; eexists.
+      sepsimpl; eexists.
+      sepsimpl; eexists.
+      sepsimpl.
+      auto.
+      all: try assumption.
+      ecancel_assumption.
+    }
+  }
+  
+      TODO: need felem copy alloc
+      simple apply compile_nlet_as_nlet_eq.
+      eapply compile_felem_small_literal_alloc; eauto.
+      simple apply compile_nlet_as_nlet_eq.
+      eapply compile_felem_small_literal_alloc; eauto.
+      apply unsigned_of_Z_1.
+      apply unsigned_of_Z_0.
+      apply unsigned_of_Z_1.
+      eapply compile_point_assign.
 (* NOTE: the plan is to completely redo montladder after ladderstep is updated to use stackalloc *)
     Abort.
 (*
